add effect soudness to small-step

theories/Meta/EffectFacts.v
@@ -9,6 +9,7 @@ Require Import theories.Core.StaticActions.
 Require Import theories.Core.Regions.
 Require Import theories.Typing.TypeSyntax.
 Require Export theories.Meta.EffectFreeVarsFacts.
+Require Import theories.Meta.RegionSubstitutionFacts.
 
 
 Lemma UnionEmptyWithEffIsEff:
@@ -16,20 +17,20 @@ Lemma UnionEmptyWithEffIsEff:
     Union_Theta (Some empty_set) eff = eff.
 Proof.
   intro.
-  induction eff; simpl; [| reflexivity]. 
+  induction eff; simpl; [| reflexivity].
   apply f_equal.
   assert (set_union empty_set a = a).
   - apply Extensionality_Ensembles.
     unfold Same_set, Included; split; intros x H_; unfold In in *.
     * destruct H_; [inversion H | assumption ].
     * apply Union_intror. assumption.
-  - assumption.    
+  - assumption.
 Qed.
 
 
 Lemma PhiInThetaTop:
   forall phi, phi ⋞ Theta_Top.
-Proof.  
+Proof.
   induction phi; intros; econstructor; try assumption; apply DAT_Top.
 Qed.
 
@@ -43,33 +44,33 @@ Proof.
   apply Extensionality_Ensembles.
   unfold Same_set, Included.
   split.
-  - intros x Hx. rewrite H1 in Hx. 
-    replace (Union ComputedAction (Empty_set ComputedAction) a) 
-    with a in Hx 
+  - intros x Hx. rewrite H1 in Hx.
+    replace (Union ComputedAction (Empty_set ComputedAction) a)
+    with a in Hx
     by (apply Extensionality_Ensembles;
-        unfold Same_set, Included; split; intros y Hy; 
+        unfold Same_set, Included; split; intros y Hy;
         unfold In in *;
           [apply Union_intror; assumption | destruct Hy; [inversion H | assumption]]).
     rewrite H2 in Hx. inversion Hx.
   - intros x Hx. inversion Hx.
-Qed. 
+Qed.
 
 Lemma EmptyUnionisEmptySet_2 :
   forall acts a,
-    Union ComputedAction acts a =  Empty_set ComputedAction -> 
+    Union ComputedAction acts a =  Empty_set ComputedAction ->
     acts = Empty_set ComputedAction /\ a = Empty_set ComputedAction.
 Proof.
   intros. split.
   + rewrite <- H.
     apply Extensionality_Ensembles.
     unfold Same_set, Included.
-    split; intros. 
+    split; intros.
     * apply Union_introl; assumption.
     * rewrite H in H0. inversion H0.
  + rewrite <- H.
    apply Extensionality_Ensembles.
    unfold Same_set, Included.
-   split; intros. 
+   split; intros.
    * apply Union_intror; assumption.
    * rewrite H in H0. inversion H0.
 Qed.
@@ -78,10 +79,10 @@ Lemma EmptyTraceIsNil:
   forall phi, phi ⋞ Theta_Empty -> phi_as_list phi = nil.
 Proof.
   induction phi; intros.
-  - reflexivity. 
-  - unfold Theta_Empty, empty_set in H. 
+  - reflexivity.
+  - unfold Theta_Empty, empty_set in H.
     dependent induction H; inversion H; subst; try (solve [inversion H2]).
-    + clear H2. clear H0. clear a. clear acts. 
+    + clear H2. clear H0. clear a. clear acts.
       dependent induction H; try (solve [inversion H]); intros.
       * eapply IHDA_in_Theta; eauto. apply EmptyUnionisEmptySet_2 in x.
         destruct x; subst. intuition.
@@ -139,18 +140,18 @@ Qed.
 
 Lemma EmptyInAnyTheta:
   forall phi theta, phi ⋞ Theta_Empty -> phi ⋞ theta .
-Proof.  
+Proof.
   induction phi; intros; try (solve [econstructor]).
   - econstructor. unfold Theta_Empty, empty_set in H.
-    dependent induction H; dependent induction H; try (solve [inversion H]). 
+    dependent induction H; dependent induction H; try (solve [inversion H]).
     * eapply IHDA_in_Theta; eauto. apply EmptyUnionisEmptySet_2 in x.
         destruct x; subst. intuition.
     * eapply IHDA_in_Theta; eauto. apply EmptyUnionisEmptySet_2 in x.
         destruct x; subst. intuition.
   - inversion H; subst.
-    apply PTS_Par; [ apply IHphi1; assumption | apply IHphi2; assumption]. 
+    apply PTS_Par; [ apply IHphi1; assumption | apply IHphi2; assumption].
   - inversion H; subst.
-    apply PTS_Seq; [ apply IHphi1; assumption | apply IHphi2; assumption]. 
+    apply PTS_Seq; [ apply IHphi1; assumption | apply IHphi2; assumption].
 Qed.
 
 Lemma EnsembleUnionSym:
@@ -160,79 +161,79 @@ Proof.
   intros phi theta theta' H.
   generalize dependent theta'.
   induction H; intros theta'.
-  - split; [apply PTS_Nil | apply PTS_Nil]. 
-  - destruct theta as [acts|]; destruct theta' as [acts'|]; 
-    intuition; simpl; try (solve [apply PTS_Elem; apply DAT_Top]). 
+  - split; [apply PTS_Nil | apply PTS_Nil].
+  - destruct theta as [acts|]; destruct theta' as [acts'|];
+    intuition; simpl; try (solve [apply PTS_Elem; apply DAT_Top]).
     + apply PTS_Elem. apply DAT_intror. assumption.
-    + apply PTS_Elem. apply DAT_introl. assumption.    
+    + apply PTS_Elem. apply DAT_introl. assumption.
   - destruct theta as [acts|]; destruct theta' as [acts'|]; intuition;
     (apply PTS_Seq; [apply IHPhi_Theta_Soundness1 | apply IHPhi_Theta_Soundness2]).
   - split; destruct theta as [acts|]; destruct theta' as [acts'|]; intuition;
-    (apply PTS_Par; [apply IHPhi_Theta_Soundness1 | apply IHPhi_Theta_Soundness2]).  
+    (apply PTS_Par; [apply IHPhi_Theta_Soundness1 | apply IHPhi_Theta_Soundness2]).
 Qed.
 
-Lemma EmptyUnionIsIdentity : 
-  forall p eff, p ⋞ (Union_Theta (Some empty_set) eff) -> p ⋞ eff. 
+Lemma EmptyUnionIsIdentity :
+  forall p eff, p ⋞ (Union_Theta (Some empty_set) eff) -> p ⋞ eff.
 Proof.
-  intros p eff H; inversion H; subst; try apply PTS_Nil.  
+  intros p eff H; inversion H; subst; try apply PTS_Nil.
   induction eff; apply PTS_Elem;
-  try assert ( HUnionEmpty : (Union_Theta (Some empty_set)  (Some a)) = Some a) 
+  try assert ( HUnionEmpty : (Union_Theta (Some empty_set)  (Some a)) = Some a)
     by (unfold Union_Theta, set_union, empty_set; f_equal;
          apply Extensionality_Ensembles; red; split; unfold Included;
          intros x Hx; [ inversion Hx; subst; [contradiction | assumption] | apply Union_intror]; auto).
   -  rewrite HUnionEmpty in H0; assumption.
-  -   apply DAT_Top. 
-  - induction eff. assert ( HUnionEmpty : (Union_Theta (Some empty_set)  (Some a)) = Some a) 
+  -   apply DAT_Top.
+  - induction eff. assert ( HUnionEmpty : (Union_Theta (Some empty_set)  (Some a)) = Some a)
      by (unfold Union_Theta, set_union, empty_set; f_equal;
          apply Extensionality_Ensembles; red; split; unfold Included;
          intros x Hx; [ inversion Hx; subst; [contradiction | assumption] | apply Union_intror]; auto).
     rewrite <- HUnionEmpty.  auto. now simpl in H.
-  -  induction eff. assert ( HUnionEmpty : (Union_Theta (Some empty_set)  (Some a)) = Some a) 
+  -  induction eff. assert ( HUnionEmpty : (Union_Theta (Some empty_set)  (Some a)) = Some a)
      by (unfold Union_Theta, set_union, empty_set; f_equal;
          apply Extensionality_Ensembles; red; split; unfold Included;
          intros x Hx; [ inversion Hx; subst; [contradiction | assumption] | apply Union_intror]; auto).
-    rewrite <- HUnionEmpty. auto. now simpl in H. 
+    rewrite <- HUnionEmpty. auto. now simpl in H.
 Qed.
 
-Lemma EmptyUnionIsIdentity_2 : 
-  forall p eff,  p ⋞ eff -> p ⋞ (Union_Theta (Some empty_set) eff). 
+Lemma EmptyUnionIsIdentity_2 :
+  forall p eff,  p ⋞ eff -> p ⋞ (Union_Theta (Some empty_set) eff).
 Proof.
-  intros p eff H; inversion H; subst; try apply PTS_Nil.  
+  intros p eff H; inversion H; subst; try apply PTS_Nil.
   induction eff; apply PTS_Elem;
-  try assert ( HUnionEmpty : (Union_Theta (Some empty_set)  (Some a)) = Some a) 
+  try assert ( HUnionEmpty : (Union_Theta (Some empty_set)  (Some a)) = Some a)
       by (unfold Union_Theta, set_union, empty_set; f_equal;
          apply Extensionality_Ensembles; red; split; unfold Included;
          intros x Hx; [ inversion Hx; subst; [contradiction | assumption] | apply Union_intror]; auto).
   - rewrite HUnionEmpty. assumption.
   - apply DAT_Top.
-  - induction eff. 
-    assert ( HUnionEmpty : (Union_Theta (Some empty_set)  (Some a)) = Some a) 
+  - induction eff.
+    assert ( HUnionEmpty : (Union_Theta (Some empty_set)  (Some a)) = Some a)
      by (unfold Union_Theta, set_union, empty_set; f_equal;
          apply Extensionality_Ensembles; red; split; unfold Included;
          intros x Hx; [ inversion Hx; subst; [contradiction | assumption] | apply Union_intror]; auto).
     + rewrite HUnionEmpty. assumption.
     + simpl. assumption.
-  - induction eff. 
-    assert ( HUnionEmpty : (Union_Theta (Some empty_set)  (Some a)) = Some a) 
+  - induction eff.
+    assert ( HUnionEmpty : (Union_Theta (Some empty_set)  (Some a)) = Some a)
      by (unfold Union_Theta, set_union, empty_set; f_equal;
          apply Extensionality_Ensembles; red; split; unfold Included;
          intros x Hx; [ inversion Hx; subst; [contradiction | assumption] | apply Union_intror]; auto).
     + rewrite HUnionEmpty. assumption.
-    + simpl. assumption.  
+    + simpl. assumption.
 Qed.
 
 Lemma EnsembleUnionComp :
   forall (phi1 phi2 : Phi) (theta1 theta2 : Theta),
     phi1 ⋞ theta1 -> phi2 ⋞ theta2 -> Phi_Seq phi1  phi2 ⋞ (Union_Theta theta1 theta2).
-Proof. 
+Proof.
   intros phi1 phi2 theta1 theta2 H1 H2.
   econstructor.
-  - apply EnsembleUnionSym with (theta' := theta2) in H1. intuition. 
+  - apply EnsembleUnionSym with (theta' := theta2) in H1. intuition.
   - apply EnsembleUnionSym with (theta' := theta1) in H2. intuition.
 Qed.
 
 
-Lemma Theta_introl: 
+Lemma Theta_introl:
   forall phi theta1 theta2, phi ⋞ theta1 -> phi ⋞ Union_Theta theta1 theta2.
 Proof.
   induction phi; intros; try (solve [econstructor]).
@@ -242,7 +243,7 @@ Proof.
                 induction theta2; [econstructor; now apply DAT_intror | econstructor; constructor ]] ).
   - apply PTS_Par. apply IHphi1. now inversion H. apply IHphi2. now inversion H.
   - apply PTS_Seq. apply IHphi1. now inversion H. apply IHphi2. now inversion H.
-Qed.    
+Qed.
 
 Lemma Theta_intror:
   forall phi theta1 theta2, phi ⋞ theta1 -> phi ⋞ Union_Theta theta2 theta1.
@@ -263,7 +264,7 @@ Lemma Disjointness_app_or_r :
     Disjoint_Traces (phi_as_list phi1) (phi_as_list phi3) \/
     Disjoint_Traces (phi_as_list phi2) (phi_as_list phi3).
 Proof.
-  intros phi1 phi2 phi3 H. 
+  intros phi1 phi2 phi3 H.
   dependent induction H.
   left; econstructor; intros.
   apply H;  [ apply in_or_app; left | ]; assumption.
@@ -275,7 +276,7 @@ Lemma Disjointness_app_or_l :
     Disjoint_Traces (phi_as_list phi1) (phi_as_list phi2) \/
     Disjoint_Traces (phi_as_list phi1) (phi_as_list phi3).
 Proof.
-  intros phi1 phi2 phi3 H. 
+  intros phi1 phi2 phi3 H.
   dependent induction H.
   left; econstructor; intros.
   apply H;  [ | apply in_or_app; left]; assumption.
@@ -287,7 +288,7 @@ Lemma Disjointness_app_app_and_r :
     Disjoint_Traces (phi_as_list phi1) (phi_as_list phi3) /\
     Disjoint_Traces (phi_as_list phi2) (phi_as_list phi3).
 Proof.
-  intros phi1 phi2 phi3 H.  
+  intros phi1 phi2 phi3 H.
   dependent induction H; split.
   - econstructor; intros. apply H;  [ apply in_or_app; left | ]; assumption.
   - econstructor; intros. apply H;  [ apply in_or_app; right | ]; assumption.
@@ -299,7 +300,7 @@ Lemma Disjointness_app_app_and_l :
     Disjoint_Traces (phi_as_list phi1) (phi_as_list phi2) /\
     Disjoint_Traces (phi_as_list phi1) (phi_as_list phi3).
 Proof.
-  intros phi1 phi2 phi3 H.  
+  intros phi1 phi2 phi3 H.
   dependent induction H; split.
   - econstructor; intros. apply H; [ |  apply in_or_app; left ]; assumption.
   - econstructor; intros. apply H;  [ | apply in_or_app; right ]; assumption.
@@ -311,7 +312,7 @@ Lemma Disjointness_and_app_r :
     Disjoint_Traces (phi_as_list phi2) (phi_as_list phi3) ->
     Disjoint_Traces (phi_as_list phi1 ++ phi_as_list phi2) (phi_as_list phi3).
 Proof.
-  intros phi1 phi2 phi3 H. destruct H. 
+  intros phi1 phi2 phi3 H. destruct H.
   generalize dependent phi2.
   dependent induction H; intros.
   econstructor; intros.
@@ -325,10 +326,10 @@ Lemma Disjointness_and_app_l :
     Disjoint_Traces (phi_as_list phi1) (phi_as_list phi3) ->
     Disjoint_Traces (phi_as_list phi1) (phi_as_list phi2 ++ phi_as_list phi3).
 Proof.
-  intros phi1 phi2 phi3 H. destruct H. 
+  intros phi1 phi2 phi3 H. destruct H.
   generalize dependent phi2.
   dependent induction H0; intros.
-  econstructor; intros. 
+  econstructor; intros.
   rename H into H1_3. inversion H0 as [? ? H1_2]; subst.
   apply in_app_or in H2; destruct H2; [apply H1_2 | apply H1_3]; auto.
 Qed.
@@ -340,10 +341,10 @@ Lemma Conflictness_app_or_l :
     Det_Trace phi3 ->
     ~ Conflict_Traces (phi_as_list phi1) (phi_as_list phi2 ++ phi_as_list phi3) ->
     ~ Conflict_Traces (phi_as_list phi1) (phi_as_list phi2) \/
-    ~ Conflict_Traces (phi_as_list phi1) (phi_as_list phi3). 
+    ~ Conflict_Traces (phi_as_list phi1) (phi_as_list phi3).
 Proof.
   intros phi1 phi2 phi3 HDet1 HDet2 HDet3 H. unfold not in *.
-  left. intro. apply H. clear H.  
+  left. intro. apply H. clear H.
   dependent induction H0;
     inversion HDet1; inversion HDet2; inversion HDet3; subst; simpl in *;
     try (solve [contradiction |
@@ -362,10 +363,10 @@ Lemma Conflictness_app_or_r :
     Det_Trace phi3 ->
     ~ Conflict_Traces (phi_as_list phi1 ++ phi_as_list phi2) (phi_as_list phi3) ->
     ~ Conflict_Traces (phi_as_list phi1) (phi_as_list phi3) \/
-    ~ Conflict_Traces (phi_as_list phi2) (phi_as_list phi3). 
+    ~ Conflict_Traces (phi_as_list phi2) (phi_as_list phi3).
 Proof.
   intros phi1 phi2 phi3 HDet1 HDet2 HDet3 H. unfold not in *.
-  left. intro. apply H. clear H.  
+  left. intro. apply H. clear H.
   dependent induction H0;
     inversion HDet1; inversion HDet2; inversion HDet3; subst; simpl in *;
     try (solve [contradiction |
@@ -385,7 +386,7 @@ Lemma Conflictness_app_and_l :
     Det_Trace phi3 ->
     ~ Conflict_Traces (phi_as_list phi1) (phi_as_list phi2 ++ phi_as_list phi3) ->
     ~ Conflict_Traces (phi_as_list phi1) (phi_as_list phi2) /\
-    ~ Conflict_Traces (phi_as_list phi1) (phi_as_list phi3). 
+    ~ Conflict_Traces (phi_as_list phi1) (phi_as_list phi3).
 Proof.
   intros phi1 phi2 phi3 HDet1 HDet2 HDet3 H. unfold not in *.
   split.
@@ -419,7 +420,7 @@ Lemma Conflictness_app_and_r :
     Det_Trace phi3 ->
     ~ Conflict_Traces (phi_as_list phi1 ++ phi_as_list phi2) (phi_as_list phi3) ->
     ~ Conflict_Traces (phi_as_list phi1) (phi_as_list phi3) /\
-    ~ Conflict_Traces (phi_as_list phi2) (phi_as_list phi3). 
+    ~ Conflict_Traces (phi_as_list phi2) (phi_as_list phi3).
 Proof.
   intros phi1 phi2 phi3 HDet1 HDet2 HDet3 H. unfold not in *.
   split.
@@ -453,7 +454,7 @@ Lemma Conflictness_or_app_l :
     Conflict_Traces (phi_as_list phi1) (phi_as_list phi2 ++ phi_as_list phi3).
 Proof.
   intros phi1 phi2 phi3 H.
-  destruct H. 
+  destruct H.
   - dependent induction H. econstructor; eauto. apply in_or_app. left; assumption.
   - dependent induction H. econstructor; eauto. apply in_or_app. right; assumption.
 Qed.
@@ -465,21 +466,21 @@ Lemma Conflictness_or_app_r :
     Conflict_Traces (phi_as_list phi1 ++ phi_as_list phi2) (phi_as_list phi3).
 Proof.
   intros phi1 phi2 phi3 H.
-  destruct H. 
+  destruct H.
   - dependent induction H. econstructor; eauto. apply in_or_app. left; assumption.
   - dependent induction H. econstructor; eauto. apply in_or_app. right; assumption.
 Qed.
- 
+
 Lemma Conflictness_and_app_l :
   forall phi1 phi2 phi3,
     ~ Conflict_Traces (phi_as_list phi1 ) (phi_as_list phi2 ) /\
     ~ Conflict_Traces (phi_as_list phi1 ) (phi_as_list phi3 ) ->
     ~ Conflict_Traces (phi_as_list phi1 ) (phi_as_list phi2  ++ phi_as_list phi3 ).
 Proof.
-  intros phi1 phi2 phi3 H. unfold not in *. destruct H. 
+  intros phi1 phi2 phi3 H. unfold not in *. destruct H.
   intro. dependent induction H1.  apply in_app_or in H3. intuition.
   + apply H. econstructor; eauto.
-  + apply H0. econstructor; eauto. 
+  + apply H0. econstructor; eauto.
 Qed.
 
 
@@ -489,10 +490,10 @@ Lemma Conflictness_and_app_r :
     ~ Conflict_Traces (phi_as_list phi2 ) (phi_as_list phi3 ) ->
     ~ Conflict_Traces (phi_as_list phi1 ++ phi_as_list phi2)  (phi_as_list phi3 ).
 Proof.
-  intros phi1 phi2 phi3 H. unfold not in *. destruct H. 
+  intros phi1 phi2 phi3 H. unfold not in *. destruct H.
   intro. dependent induction H1.  apply in_app_or in H3. intuition.
   + apply H. econstructor; eauto.
-  + apply H0. econstructor; eauto. 
+  + apply H0. econstructor; eauto.
 Qed.
 
 
@@ -519,8 +520,358 @@ Inductive Epsilon_Phi_Soundness :  (Epsilon * Phi) -> Prop :=
                            /\ SA_DA_Soundness sa da) ->
     Epsilon_Phi_Soundness (st, dy).
 
+Definition DynamicAction_StaticAction (da : DynamicAction) : StaticAction :=
+  match da with
+  | DA_Alloc r _ _ => SA_Alloc (Rgn_Const true true r)
+  | DA_Read r _ _ => SA_Read (Rgn_Const true true r)
+  | DA_Write r _ _ => SA_Write (Rgn_Const true true r)
+  end.
 
-Lemma ReadOnlyStaticImpliesReadOnlySubstStatic : 
+Definition DynamicAction_Epsilon (da : DynamicAction) : Epsilon :=
+  Singleton_Static_Action (DynamicAction_StaticAction da).
+
+Fixpoint Phi_Static_Effect (phi : Phi) : Epsilon :=
+  match phi with
+  | Phi_Nil => Empty_Static_Action
+  | Phi_Elem da => DynamicAction_Epsilon da
+  | Phi_Par phi1 phi2 =>
+      Union_Static_Action (Phi_Static_Effect phi1) (Phi_Static_Effect phi2)
+  | Phi_Seq phi1 phi2 =>
+      Union_Static_Action (Phi_Static_Effect phi1) (Phi_Static_Effect phi2)
+  end.
+
+Lemma DynamicAction_StaticAction_sound :
+  forall da,
+    SA_DA_Soundness (DynamicAction_StaticAction da) da.
+Proof.
+  intros da.
+  destruct da; constructor.
+Qed.
+
+Lemma Epsilon_Phi_Soundness_nil :
+  forall eps,
+    Epsilon_Phi_Soundness (eps, Phi_Nil).
+Proof.
+  intros eps.
+  constructor.
+  intros da HIn.
+  inversion HIn.
+Qed.
+
+Lemma Epsilon_Phi_Soundness_elem :
+  forall da,
+    Epsilon_Phi_Soundness (DynamicAction_Epsilon da, Phi_Elem da).
+Proof.
+  intros da.
+  constructor.
+  intros da' HIn.
+  inversion HIn; subst.
+  exists (DynamicAction_StaticAction da).
+  split.
+  - apply Ensembles.In_singleton.
+  - apply DynamicAction_StaticAction_sound.
+Qed.
+
+Lemma Epsilon_Phi_Soundness_seq :
+  forall eps1 eps2 phi1 phi2,
+    Epsilon_Phi_Soundness (eps1, phi1) ->
+    Epsilon_Phi_Soundness (eps2, phi2) ->
+    Epsilon_Phi_Soundness
+      (Union_Static_Action eps1 eps2, Phi_Seq phi1 phi2).
+Proof.
+  intros eps1 eps2 phi1 phi2 H1 H2.
+  inversion H1 as [? ? HEps1]; inversion H2 as [? ? HEps2]; subst.
+  constructor.
+  intros da HIn.
+  inversion HIn; subst.
+  destruct H3 as [HIn1 | HIn2].
+  - destruct (HEps1 da HIn1) as [sa [HInSa HSound]].
+    exists sa.
+    split; [apply Ensembles.Union_introl; assumption | assumption].
+  - destruct (HEps2 da HIn2) as [sa [HInSa HSound]].
+    exists sa.
+    split; [apply Ensembles.Union_intror; assumption | assumption].
+Qed.
+
+Lemma Epsilon_Phi_Soundness_par :
+  forall eps1 eps2 phi1 phi2,
+    Epsilon_Phi_Soundness (eps1, phi1) ->
+    Epsilon_Phi_Soundness (eps2, phi2) ->
+    Epsilon_Phi_Soundness
+      (Union_Static_Action eps1 eps2, Phi_Par phi1 phi2).
+Proof.
+  intros eps1 eps2 phi1 phi2 H1 H2.
+  inversion H1 as [? ? HEps1]; inversion H2 as [? ? HEps2]; subst.
+  constructor.
+  intros da HIn.
+  inversion HIn; subst.
+  destruct H3 as [HIn1 | HIn2].
+  - destruct (HEps1 da HIn1) as [sa [HInSa HSound]].
+    exists sa.
+    split; [apply Ensembles.Union_introl; assumption | assumption].
+  - destruct (HEps2 da HIn2) as [sa [HInSa HSound]].
+    exists sa.
+    split; [apply Ensembles.Union_intror; assumption | assumption].
+Qed.
+
+Theorem Phi_Static_Effect_sound :
+  forall phi,
+    Epsilon_Phi_Soundness (Phi_Static_Effect phi, phi).
+Proof.
+  induction phi.
+  - apply Epsilon_Phi_Soundness_nil.
+  - apply Epsilon_Phi_Soundness_elem.
+  - simpl. apply Epsilon_Phi_Soundness_par; assumption.
+  - simpl. apply Epsilon_Phi_Soundness_seq; assumption.
+Qed.
+
+Lemma Epsilon_Phi_Soundness_weaken :
+  forall eps1 eps2 phi,
+    Included StaticAction eps1 eps2 ->
+    Epsilon_Phi_Soundness (eps1, phi) ->
+    Epsilon_Phi_Soundness (eps2, phi).
+Proof.
+  intros eps1 eps2 phi HIncluded HSound.
+  inversion HSound as [? ? HEps]; subst.
+  constructor.
+  intros da HIn.
+  destruct (HEps da HIn) as [sa [HInSa HSoundSa]].
+  exists sa.
+  split; [apply HIncluded; assumption | assumption].
+Qed.
+
+Lemma SA_DA_Soundness_static_unique :
+  forall sa da,
+    SA_DA_Soundness sa da ->
+    sa = DynamicAction_StaticAction da.
+Proof.
+  intros sa da HSound.
+  inversion HSound; reflexivity.
+Qed.
+
+Theorem Phi_Static_Effect_least :
+  forall phi eps,
+    Epsilon_Phi_Soundness (eps, phi) ->
+    Included StaticAction (Phi_Static_Effect phi) eps.
+Proof.
+  induction phi; intros eps HSound; simpl; unfold Included; intros sa HIn.
+  - inversion HIn.
+  - unfold DynamicAction_Epsilon, Singleton_Static_Action in HIn.
+    inversion HIn; subst.
+    inversion HSound as [? ? HEps]; subst.
+    destruct (HEps d (DAP_Trace d)) as [sa' [HInSa HSoundSa]].
+    pose proof (SA_DA_Soundness_static_unique sa' d HSoundSa) as HUnique.
+    subst sa'.
+    exact HInSa.
+  - inversion HSound as [? ? HEps]; subst.
+    destruct HIn as [sa HInLeft | sa HInRight].
+    + eapply IHphi1; [| exact HInLeft].
+      constructor.
+      intros da HDA.
+      apply HEps.
+      apply DAP_Par.
+      left. exact HDA.
+    + eapply IHphi2; [| exact HInRight].
+      constructor.
+      intros da HDA.
+      apply HEps.
+      apply DAP_Par.
+      right. exact HDA.
+  - inversion HSound as [? ? HEps]; subst.
+    destruct HIn as [sa HInLeft | sa HInRight].
+    + eapply IHphi1; [| exact HInLeft].
+      constructor.
+      intros da HDA.
+      apply HEps.
+      apply DAP_Seq.
+      left. exact HDA.
+    + eapply IHphi2; [| exact HInRight].
+      constructor.
+      intros da HDA.
+      apply HEps.
+      apply DAP_Seq.
+      right. exact HDA.
+Qed.
+
+Theorem Epsilon_Phi_Soundness_of_phi_static_included :
+  forall eps phi,
+    Included StaticAction (Phi_Static_Effect phi) eps ->
+    Epsilon_Phi_Soundness (eps, phi).
+Proof.
+  intros eps phi HIncluded.
+  eapply Epsilon_Phi_Soundness_weaken.
+  - exact HIncluded.
+  - apply Phi_Static_Effect_sound.
+Qed.
+
+Theorem Epsilon_Phi_Soundness_iff_phi_static_included :
+  forall eps phi,
+    Epsilon_Phi_Soundness (eps, phi) <->
+    Included StaticAction (Phi_Static_Effect phi) eps.
+Proof.
+  intros eps phi.
+  split.
+  - intros HSound.
+    apply Phi_Static_Effect_least.
+    exact HSound.
+  - intros HIncluded.
+    apply Epsilon_Phi_Soundness_of_phi_static_included.
+    exact HIncluded.
+Qed.
+
+Lemma fold_dist_union :
+  forall rho (eff1 eff2 : Epsilon),
+    fold_subst_eps rho (Union_Static_Action eff1 eff2) =
+    Union_Static_Action (fold_subst_eps rho eff1) (fold_subst_eps rho eff2).
+Proof.
+  intros rho eff1 eff2.
+  unfold fold_subst_eps.
+  apply Extensionality_Ensembles.
+  unfold Same_set, Included.
+  split; intros sa HIn; unfold Ensembles.In in *.
+  - destruct HIn as [sa' [HIn HSubst]].
+    subst.
+    destruct HIn as [sa' HInLeft | sa' HInRight].
+    + apply Union_introl.
+      exists sa'. split; [assumption | reflexivity].
+    + apply Union_intror.
+      exists sa'. split; [assumption | reflexivity].
+  - destruct HIn as [sa HInLeft | sa HInRight].
+    + destruct HInLeft as [sa' [HInLeft HSubst]].
+      subst.
+      exists sa'. split; [apply Union_introl; assumption | reflexivity].
+    + destruct HInRight as [sa' [HInRight HSubst]].
+      subst.
+      exists sa'. split; [apply Union_intror; assumption | reflexivity].
+Qed.
+
+Lemma fold_subst_rgn_mk_rgn_type_find_R :
+  forall rho w r,
+    find_R w rho = Some r ->
+    fold_subst_rgn rho (mk_rgn_type w) = Rgn_Const true true r.
+Proof.
+  intros rho w r HFind.
+  unfold find_R in HFind.
+  unfold mk_rgn_type.
+  destruct w; simpl in HFind.
+  - inversion HFind; subst.
+    simpl.
+    apply subst_rho_rgn_const.
+  - simpl.
+    eapply subst_rho_fvar_2; eauto.
+  - discriminate.
+Qed.
+
+Lemma fold_subst_eps_singleton_alloc_find_R :
+  forall rho w r,
+    find_R w rho = Some r ->
+    Ensembles.In StaticAction
+      (fold_subst_eps rho
+        (Singleton_Static_Action (SA_Alloc (mk_rgn_type w))))
+      (SA_Alloc (Rgn_Const true true r)).
+Proof.
+  intros rho w r HFind.
+  unfold fold_subst_eps.
+  exists (SA_Alloc (mk_rgn_type w)).
+  split.
+  - apply Ensembles.In_singleton.
+  - unfold fold_subst_sa.
+    f_equal.
+    eapply fold_subst_rgn_mk_rgn_type_find_R; eauto.
+Qed.
+
+Lemma fold_subst_eps_singleton_read_find_R :
+  forall rho w r,
+    find_R w rho = Some r ->
+    Ensembles.In StaticAction
+      (fold_subst_eps rho
+        (Singleton_Static_Action (SA_Read (mk_rgn_type w))))
+      (SA_Read (Rgn_Const true true r)).
+Proof.
+  intros rho w r HFind.
+  unfold fold_subst_eps.
+  exists (SA_Read (mk_rgn_type w)).
+  split.
+  - apply Ensembles.In_singleton.
+  - unfold fold_subst_sa.
+    f_equal.
+    eapply fold_subst_rgn_mk_rgn_type_find_R; eauto.
+Qed.
+
+Lemma fold_subst_eps_singleton_write_find_R :
+  forall rho w r,
+    find_R w rho = Some r ->
+    Ensembles.In StaticAction
+      (fold_subst_eps rho
+        (Singleton_Static_Action (SA_Write (mk_rgn_type w))))
+      (SA_Write (Rgn_Const true true r)).
+Proof.
+  intros rho w r HFind.
+  unfold fold_subst_eps.
+  exists (SA_Write (mk_rgn_type w)).
+  split.
+  - apply Ensembles.In_singleton.
+  - unfold fold_subst_sa.
+    f_equal.
+    eapply fold_subst_rgn_mk_rgn_type_find_R; eauto.
+Qed.
+
+Lemma Epsilon_Phi_Soundness_alloc_find_R :
+  forall rho w r l v,
+    find_R w rho = Some r ->
+    Epsilon_Phi_Soundness
+      (fold_subst_eps rho
+        (Singleton_Static_Action (SA_Alloc (mk_rgn_type w))),
+       Phi_Elem (DA_Alloc r l v)).
+Proof.
+  intros rho w r l v HFind.
+  constructor.
+  intros da HIn.
+  inversion HIn; subst.
+  exists (SA_Alloc (Rgn_Const true true r)).
+  split.
+  - eapply fold_subst_eps_singleton_alloc_find_R; eauto.
+  - constructor.
+Qed.
+
+Lemma Epsilon_Phi_Soundness_read_find_R :
+  forall rho w r l v,
+    find_R w rho = Some r ->
+    Epsilon_Phi_Soundness
+      (fold_subst_eps rho
+        (Singleton_Static_Action (SA_Read (mk_rgn_type w))),
+       Phi_Elem (DA_Read r l v)).
+Proof.
+  intros rho w r l v HFind.
+  constructor.
+  intros da HIn.
+  inversion HIn; subst.
+  exists (SA_Read (Rgn_Const true true r)).
+  split.
+  - eapply fold_subst_eps_singleton_read_find_R; eauto.
+  - constructor.
+Qed.
+
+Lemma Epsilon_Phi_Soundness_write_find_R :
+  forall rho w r l v,
+    find_R w rho = Some r ->
+    Epsilon_Phi_Soundness
+      (fold_subst_eps rho
+        (Singleton_Static_Action (SA_Write (mk_rgn_type w))),
+       Phi_Elem (DA_Write r l v)).
+Proof.
+  intros rho w r l v HFind.
+  constructor.
+  intros da HIn.
+  inversion HIn; subst.
+  exists (SA_Write (Rgn_Const true true r)).
+  split.
+  - eapply fold_subst_eps_singleton_write_find_R; eauto.
+  - constructor.
+Qed.
+
+
+Lemma ReadOnlyStaticImpliesReadOnlySubstStatic :
   forall eps rho,
     ReadOnlyStatic eps ->
     ReadOnlyStatic (fold_subst_eps rho eps).
@@ -546,9 +897,9 @@ Proof.
     unfold Same_set, Included; split; intros x H; unfold Ensembles.In in *.
     + inversion H; subst; inversion H0; unfold fold_subst_eps; exists x0; split.
       * apply Ensembles.Union_introl. destruct H1; subst. assumption.
-      * destruct H1; subst. reflexivity. 
+      * destruct H1; subst. reflexivity.
       * apply Ensembles.Union_intror. destruct H1; subst. assumption.
-      * destruct H1; subst. reflexivity.   
+      * destruct H1; subst. reflexivity.
    + inversion H. inversion H0. inversion H1; subst;
        [apply Ensembles.Union_introl | apply Ensembles.Union_intror];
        unfold Ensembles.In; unfold fold_subst_eps; exists x0.
@@ -566,7 +917,7 @@ Proof.
   - constructor.
   - induction d.
     + exfalso; induction ROS.
-      * inversion H; subst. 
+      * inversion H; subst.
         edestruct H1; [econstructor | destruct H0 ; inversion H0].
       * inversion H; subst.
         edestruct H1; [econstructor | destruct H0 ; inversion H0; subst; inversion H2 ].
@@ -576,7 +927,7 @@ Proof.
         apply IHROS2; constructor; intros; inversion H4; subst; exists x; intuition.
     + econstructor.
     + exfalso; induction ROS.
-      * inversion H; subst. 
+      * inversion H; subst.
         edestruct H1; [econstructor | destruct H0 ; inversion H0].
       * inversion H; subst.
         edestruct H1; [econstructor | destruct H0 ; inversion H0; subst; inversion H2 ].
@@ -595,4 +946,3 @@ Proof.
     constructor; intros da daIn; inversion H; subst; apply (H2 da); apply DAP_Seq; auto.
     constructor; auto.
 Qed.
-
